---
title: 'Chapter 5: Normal Distrbution'
author: 'Shao-Ting Chiu'
date: '20220901'
jupyter: 'r'
execute: 
  freeze: auto
---

## The normal model

$$p(y|\theta, \sigma^2) = \frac{1}{\sigma\sqrt{2\pi}}e^{\frac{-1}{2}(\frac{y-\theta}{\sigma})^2}, \quad -\infty < y < \infty$$

## Total Expectation and variance

- Iterative Expectation
$$E(X) = E(E(X|\omega))$$

- Iterative Variance
$$Var(X) = E(Var(X|\omega)) + Var(E(X|\omega))$$

## Joint inference for mean and prediction



## Jeffreys prior



\begin{equation}
  I(\theta_1, \theta_2) = 
  \begin{pmatrix}
    \theta_2 & 0\\ 
    0 & .5\theta_{2}^{-2}
  \end{pmatrix}
\end{equation}

Derivation:

$$l(\theta)=\log(y|\theta) = -.5\log(2\pi)+.5\log(\theta_2) - .5 \theta_2(y-\theta_1)^2$$

$$\frac{\partial l(\theta)}{\partial \theta_1} = \theta_2(y-\theta_1), \frac{\partial l(\theta)}{\partial \theta^{2}_{1}}=-\theta_2$$


$$\frac{\partial^2 l(\theta)}{\partial\theta_2\partial\theta_1} = y - \theta_1$$

$$\frac{\partial l(\theta)}{\partial \theta_2} = .5\theta^{-1}_{2} - .5 (y-\theta_1)^2, \frac{\partial^2 l(\theta)}{\partial \theta_{2}^{2}} = -.5\theta_{2}^{-2}$$